\documentclass[fleqn]{IEEEtran}

\usepackage{amsmath}
\usepackage{amsfonts}

\begin{document}

\section{Overview}

	Given:

	\begin{equation}
		y = \Delta{}t + \Delta{}v
	\end{equation}
	
\section{Time-Domain}

	Since:

	\begin{equation}
		\Delta{}t = \frac{d_{\vec{ms}}}{c}
	\end{equation}
	
	Where:

	\begin{equation}
		c = 343 \pm c_{\text{adj}}
	\end{equation}
	
	\begin{equation}
		c_{\text{adj}} = [0, 10]
	\end{equation}
	
	\begin{equation}
		\Delta{}D_{\vec{ms}} = \sqrt{(x_s - x_m)^2 + (y_s - y_m)^2}
	\end{equation}
	
	Thus:
	
	\begin{equation}
		\Delta{}t = \frac{
			\sqrt{(x_s - x_m)^2 + (y_s - y_m)^2}
			}
			{
			343 \pm [0,10]
			}
	\end{equation}
	
\section{Amplitude-Domain}
	
	If:

	\begin{equation}
		\begin{bmatrix} W \\ X \\ Y \end{bmatrix} = S *  \begin{bmatrix} \sqrt{2} \\ \cos{\Theta{}_s}\\ \sin{\Theta{}_s} \end{bmatrix}
	\end{equation}
	
	And:
	
	\begin{equation}
		m(\Theta, p) = (1-p)m_\text{omni} + pm_\text{bi}
	\end{equation}
	
	Where:
	
	\begin{equation}
		m_\text{omni} = 1
	\end{equation}
	
	And:
	
	\begin{equation}
		m_\text{bi} = \sin{\Theta_m} + \cos{\Theta_m }
	\end{equation}
	
	Then:
	
	\begin{equation}
		\Delta{}v = \begin{bmatrix} W \\ X \\ Y \end{bmatrix} * m(\Theta, p)
	\end{equation}
	
	Which is:
	
	\begin{equation}
		\Delta{}v = S(1 - p)\sqrt{2} + p(S\sin{\Theta_m}\sin{\Theta_s} + S\cos{\Theta_m}\cos{\Theta_s})
	\end{equation}
	
	However:
	
	\begin{equation}
		\Delta{}v = S(1 - p)\sqrt{2} + pS(\cos{(\Theta_m - \Theta_s)})
	\end{equation}
	
	Which is:
	
	\begin{equation}
		\Delta{}v = S[(1-p)\sqrt(2) + p(\cos{(\Theta_m - \Theta_s)})]
	\end{equation}
	
	Thus:
	
	\begin{equation}
		m(\Theta_{m-s}, p) = (1-p)\sqrt{2} + p\cos{\Theta}
	\end{equation}
	
	And:
	
	\begin{equation}
		\Delta{}v = S * m(\Theta_{m-s}, p)
	\end{equation}

\section{Conclusion}

Therefore:

	\begin{equation}
		y[n] = n((1-p)\sqrt{2} + p\cos{\Theta}) + \hat{t}\frac{
			\sqrt{(x_s - x_m)^2 + (y_s - y_m)^2}
			}
			{
			343 \pm [0,10]
			}
	\end{equation}

\end{document}